

MA579H Scientific Computing

Polynomial Interpolation-II

Rafikul Alam
Department of Mathematics
IIT Guwahati

Lecture outline

- Newton interpolating polynomial
- Divided difference

Newton interpolating polynomial

Example: For the data set $(x_0, f_0), (x_1, f_1), (x_2, f_2)$, consider **Newton polynomial** $p(x) = a_0 + a_1(x - x_0) + a_2(x - x_0)(x - x_1)$.

Newton interpolating polynomial

Example: For the data set $(x_0, f_0), (x_1, f_1), (x_2, f_2)$, consider **Newton polynomial** $p(x) = a_0 + a_1(x - x_0) + a_2(x - x_0)(x - x_1)$. Then the conditions $p(x_0) = f_0, p(x_1) = f_1, p(x_2) = f_2$ yield

$$\begin{bmatrix} 1 & 0 & 0 \\ 1 & (x_1 - x_0) & 0 \\ 1 & (x_2 - x_0) & (x_2 - x_0)(x_2 - x_1) \end{bmatrix} \begin{bmatrix} a_0 \\ a_1 \\ a_2 \end{bmatrix} = \begin{bmatrix} f_0 \\ f_1 \\ f_2 \end{bmatrix}.$$

Newton interpolating polynomial

Example: For the data set $(x_0, f_0), (x_1, f_1), (x_2, f_2)$, consider **Newton polynomial** $p(x) = a_0 + a_1(x - x_0) + a_2(x - x_0)(x - x_1)$. Then the conditions $p(x_0) = f_0, p(x_1) = f_1, p(x_2) = f_2$ yield

$$\begin{bmatrix} 1 & 0 & 0 \\ 1 & (x_1 - x_0) & 0 \\ 1 & (x_2 - x_0) & (x_2 - x_0)(x_2 - x_1) \end{bmatrix} \begin{bmatrix} a_0 \\ a_1 \\ a_2 \end{bmatrix} = \begin{bmatrix} f_0 \\ f_1 \\ f_2 \end{bmatrix}.$$

For the data set $(-2, -27), (0, -1), (1, 0)$, we have

$$\begin{bmatrix} 1 & 0 & 0 \\ 1 & 2 & 0 \\ 1 & 3 & 3 \end{bmatrix} \begin{bmatrix} a_0 \\ a_1 \\ a_2 \end{bmatrix} = \begin{bmatrix} -27 \\ -1 \\ 0 \end{bmatrix} \implies [a_0, a_1, a_2] = [-27, 13, -4].$$

Hence $p(x) = -27 + 13(x + 2) - 4(x + 2)x = -1 + 5x - 4x^2$.

Newton interpolating polynomial

Define $N_0(x) := 1$ and $N_j(x) := (x - x_0) \cdots (x - x_{j-1})$ for $j = 1 : n$.
Then $N_j(x_i) = 0$ for $i = 0 : j - 1$ and $j = 1 : n$.

Newton interpolating polynomial

Define $N_0(x) := 1$ and $N_j(x) := (x - x_0) \cdots (x - x_{j-1})$ for $j = 1 : n$.
Then $N_j(x_i) = 0$ for $i = 0 : j - 1$ and $j = 1 : n$.

Note that $N_{j+1}(x) = N_j(x)(x - x_j)$ for $j = 1 : n - 1$.

Newton interpolating polynomial

Define $N_0(x) := 1$ and $N_j(x) := (x - x_0) \cdots (x - x_{j-1})$ for $j = 1 : n$.
Then $N_j(x_i) = 0$ for $i = 0 : j - 1$ and $j = 1 : n$.

Note that $N_{j+1}(x) = N_j(x)(x - x_j)$ for $j = 1 : n - 1$.

Fact: The Newton polynomials $N_0(x), \dots, N_n(x)$ form a basis of \mathcal{P}_n which is referred to as **Newton basis**.

Let $p(x) := a_0 N_0(x) + \cdots + a_n N_n(x)$. The interpolation conditions $p(x_j) = f_j$ for $j = 0 : n$ yield the **lower triangular system**

Newton interpolating polynomial

Define $N_0(x) := 1$ and $N_j(x) := (x - x_0) \cdots (x - x_{j-1})$ for $j = 1 : n$.
Then $N_j(x_i) = 0$ for $i = 0 : j - 1$ and $j = 1 : n$.

Note that $N_{j+1}(x) = N_j(x)(x - x_j)$ for $j = 1 : n - 1$.

Fact: The Newton polynomials $N_0(x), \dots, N_n(x)$ form a basis of \mathcal{P}_n which is referred to as **Newton basis**.

Let $p(x) := a_0 N_0(x) + \cdots + a_n N_n(x)$. The interpolation conditions $p(x_j) = f_j$ for $j = 0 : n$ yield the **lower triangular system**

$$\begin{bmatrix} N_0(x_0) & 0 & 0 & \cdots & 0 \\ N_0(x_1) & N_1(x_1) & 0 & \cdots & 0 \\ N_0(x_2) & N_1(x_2) & N_2(x_2) & \cdots & 0 \\ \vdots & \vdots & \vdots & \ddots & \vdots \\ N_0(x_n) & N_1(x_n) & N_2(x_n) & \cdots & N_n(x_n) \end{bmatrix} \begin{bmatrix} a_0 \\ a_1 \\ a_2 \\ \vdots \\ a_n \end{bmatrix} = \begin{bmatrix} f_0 \\ f_1 \\ f_2 \\ \vdots \\ f_n \end{bmatrix}.$$

Newton interpolating polynomial

Define $N_0(x) := 1$ and $N_j(x) := (x - x_0) \cdots (x - x_{j-1})$ for $j = 1 : n$.
Then $N_j(x_i) = 0$ for $i = 0 : j - 1$ and $j = 1 : n$.

Note that $N_{j+1}(x) = N_j(x)(x - x_j)$ for $j = 1 : n - 1$.

Fact: The Newton polynomials $N_0(x), \dots, N_n(x)$ form a basis of \mathcal{P}_n which is referred to as **Newton basis**.

Let $p(x) := a_0 N_0(x) + \cdots + a_n N_n(x)$. The interpolation conditions $p(x_j) = f_j$ for $j = 0 : n$ yield the **lower triangular system**

$$\begin{bmatrix} N_0(x_0) & 0 & 0 & \cdots & 0 \\ N_0(x_1) & N_1(x_1) & 0 & \cdots & 0 \\ N_0(x_2) & N_1(x_2) & N_2(x_2) & \cdots & 0 \\ \vdots & \vdots & \vdots & \ddots & \vdots \\ N_0(x_n) & N_1(x_n) & N_2(x_n) & \cdots & N_n(x_n) \end{bmatrix} \begin{bmatrix} a_0 \\ a_1 \\ a_2 \\ \vdots \\ a_n \end{bmatrix} = \begin{bmatrix} f_0 \\ f_1 \\ f_2 \\ \vdots \\ f_n \end{bmatrix}.$$

Solving the triangular system for $a_j, j = 0 : n$, we obtain the interpolating polynomial $p(x) = a_0 N_0(x) + \cdots + a_n N_n(x)$ in **Newton's form**.

Newton interpolating polynomial

Remark:

- Solution of the lower triangular system requires $\mathcal{O}(n^2)$ flops.
- Computation of $p(x)$ requires $\mathcal{O}(n^2)$ operations.
- Can accommodate new data (x_{n+1}, f_{n+1}) with additional $\mathcal{O}(n)$ operations.
- Evaluation of $p(x)$ at a given x requires $\mathcal{O}(n^2)$ operations.

Computation of $N_j(x_j)$ may be prone to overflow/underflow. However, $p(x)$ can be computed more efficiently using divided difference table.

Divided differences

Consider the data set $(x_0, f_0), \dots, (x_n, f_n)$. Define

$$\begin{aligned} f[x_j] &:= f_j \text{ for } j = 0 : n, \\ f[x_0, x_1] &:= \frac{f[x_1] - f[x_0]}{x_1 - x_0} \end{aligned}$$

Divided differences

Consider the data set $(x_0, f_0), \dots, (x_n, f_n)$. Define

$$\begin{aligned}f[x_j] &:= f_j \text{ for } j = 0 : n, \\f[x_0, x_1] &:= \frac{f[x_1] - f[x_0]}{x_1 - x_0} \\f[x_0, x_1, x_2] &:= \frac{f[x_1, x_2] - f[x_0, x_1]}{x_2 - x_0} \\&\vdots \\f[x_0, x_1, \dots, x_n] &:= \frac{f[x_1, x_2, \dots, x_n] - f[x_0, x_1, \dots, x_{n-1}]}{x_n - x_0}\end{aligned}$$

Divided differences

Consider the data set $(x_0, f_0), \dots, (x_n, f_n)$. Define

$$\begin{aligned} f[x_j] &:= f_j \text{ for } j = 0 : n, \\ f[x_0, x_1] &:= \frac{f[x_1] - f[x_0]}{x_1 - x_0} \\ f[x_0, x_1, x_2] &:= \frac{f[x_1, x_2] - f[x_0, x_1]}{x_2 - x_0} \\ &\vdots \\ f[x_0, x_1, \dots, x_n] &:= \frac{f[x_1, x_2, \dots, x_n] - f[x_0, x_1, \dots, x_{n-1}]}{x_n - x_0} \end{aligned}$$

The divided differences can **update new data** (x_{n+1}, f_{n+1}) with $\mathcal{O}(n)$ additional operations.

Newton interpolating polynomial

Consider $(x_0, f_0), (x_1, f_1), (x_2, f_2)$ and the Newton polynomial $p(x) = a_0 + a_1(x - x_0) + a_2(x - x_0)(x - x_1)$. Set $f[x_j] := f_j$ for $j = 0, 1, 2$. Then $p(x_0) = f_0, p(x_1) = f_1$ and $p(x_2) = f_2$ yield

$$a_0 = f_0 = f[x_0]$$

Newton interpolating polynomial

Consider $(x_0, f_0), (x_1, f_1), (x_2, f_2)$ and the Newton polynomial $p(x) = a_0 + a_1(x - x_0) + a_2(x - x_0)(x - x_1)$. Set $f[x_j] := f_j$ for $j = 0, 1, 2$. Then $p(x_0) = f_0, p(x_1) = f_1$ and $p(x_2) = f_2$ yield

$$\begin{aligned}a_0 &= f_0 = f[x_0] \\a_1 &= \frac{f[x_1] - f[x_0]}{x_1 - x_0} = f[x_0, x_1]\end{aligned}$$

Newton interpolating polynomial

Consider $(x_0, f_0), (x_1, f_1), (x_2, f_2)$ and the Newton polynomial $p(x) = a_0 + a_1(x - x_0) + a_2(x - x_0)(x - x_1)$. Set $f[x_j] := f_j$ for $j = 0, 1, 2$. Then $p(x_0) = f_0, p(x_1) = f_1$ and $p(x_2) = f_2$ yield

$$a_0 = f_0 = f[x_0]$$

$$a_1 = \frac{f[x_1] - f[x_0]}{x_1 - x_0} = f[x_0, x_1]$$

$$a_2 = \left(\frac{f[x_2] - f[x_0]}{x_2 - x_0} - f[x_0, x_1] \right) / (x_2 - x_1)$$

Newton interpolating polynomial

Consider $(x_0, f_0), (x_1, f_1), (x_2, f_2)$ and the Newton polynomial $p(x) = a_0 + a_1(x - x_0) + a_2(x - x_0)(x - x_1)$. Set $f[x_j] := f_j$ for $j = 0, 1, 2$. Then $p(x_0) = f_0, p(x_1) = f_1$ and $p(x_2) = f_2$ yield

$$a_0 = f_0 = f[x_0]$$

$$a_1 = \frac{f[x_1] - f[x_0]}{x_1 - x_0} = f[x_0, x_1]$$

$$\begin{aligned} a_2 &= \left(\frac{f[x_2] - f[x_0]}{x_2 - x_0} - f[x_0, x_1] \right) / (x_2 - x_1) \\ &= \left(\frac{f[x_2] - f[x_1]}{x_2 - x_0} + \frac{f[x_1] - f[x_0]}{x_2 - x_0} - f[x_0, x_1] \right) / (x_2 - x_1) \end{aligned}$$

Newton interpolating polynomial

Consider $(x_0, f_0), (x_1, f_1), (x_2, f_2)$ and the Newton polynomial $p(x) = a_0 + a_1(x - x_0) + a_2(x - x_0)(x - x_1)$. Set $f[x_j] := f_j$ for $j = 0, 1, 2$. Then $p(x_0) = f_0, p(x_1) = f_1$ and $p(x_2) = f_2$ yield

$$a_0 = f_0 = f[x_0]$$

$$a_1 = \frac{f[x_1] - f[x_0]}{x_1 - x_0} = f[x_0, x_1]$$

$$\begin{aligned} a_2 &= \left(\frac{f[x_2] - f[x_0]}{x_2 - x_0} - f[x_0, x_1] \right) / (x_2 - x_1) \\ &= \left(\frac{f[x_2] - f[x_1]}{x_2 - x_0} + \frac{f[x_1] - f[x_0]}{x_2 - x_0} - f[x_0, x_1] \right) / (x_2 - x_1) \\ &= \frac{f[x_1, x_2] - f[x_0, x_1]}{x_2 - x_0} = f[x_0, x_1, x_2] \end{aligned}$$

Newton interpolating polynomial

Consider $(x_0, f_0), (x_1, f_1), (x_2, f_2)$ and the Newton polynomial $p(x) = a_0 + a_1(x - x_0) + a_2(x - x_0)(x - x_1)$. Set $f[x_j] := f_j$ for $j = 0, 1, 2$. Then $p(x_0) = f_0, p(x_1) = f_1$ and $p(x_2) = f_2$ yield

$$\begin{aligned}a_0 &= f_0 = f[x_0] \\a_1 &= \frac{f[x_1] - f[x_0]}{x_1 - x_0} = f[x_0, x_1] \\a_2 &= \left(\frac{f[x_2] - f[x_0]}{x_2 - x_0} - f[x_0, x_1] \right) / (x_2 - x_1) \\&= \left(\frac{f[x_2] - f[x_1]}{x_2 - x_0} + \frac{f[x_1] - f[x_0]}{x_2 - x_0} - f[x_0, x_1] \right) / (x_2 - x_1) \\&= \frac{f[x_1, x_2] - f[x_0, x_1]}{x_2 - x_0} = f[x_0, x_1, x_2]\end{aligned}$$

This shows that

$$p(x) = f[x_0] + f[x_0, x_1](x - x_0) + f[x_0, x_1, x_2](x - x_0)(x - x_1).$$

Divided differences table

Divided differences can be generated by using the [table of divided differences](#):

x	f				
x_0	f_0				
x_1	f_1	$f[x_0, x_1]$			
x_2	f_2	$f[x_1, x_2]$	$f[x_0, x_1, x_2]$		
x_3	f_3	$f[x_2, x_3]$	$f[x_1, x_2, x_3]$	$f[x_0, x_1, x_2, x_3]$	
\cdot	\cdot	\dots	\dots	\dots	

Divided differences table

Divided differences can be generated by using the [table of divided differences](#):

x	f				
x_0	f_0				
x_1	f_1	$f[x_0, x_1]$			
x_2	f_2	$f[x_1, x_2]$	$f[x_0, x_1, x_2]$		
x_3	f_3	$f[x_2, x_3]$	$f[x_1, x_2, x_3]$	$f[x_0, x_1, x_2, x_3]$	
\cdot	\cdot	\dots	\dots	\dots	

The $n + 1$ diagonal entries in the table of divided differences are the coefficients of the Newton interpolating polynomial $p(x)$.

Divided differences table

Divided differences can be generated by using the [table of divided differences](#):

x	f				
x_0	f_0				
x_1	f_1	$f[x_0, x_1]$			
x_2	f_2	$f[x_1, x_2]$	$f[x_0, x_1, x_2]$		
x_3	f_3	$f[x_2, x_3]$	$f[x_1, x_2, x_3]$	$f[x_0, x_1, x_2, x_3]$	
\cdot	\cdot	\dots	\dots	\dots	

The $n + 1$ diagonal entries in the table of divided differences are the coefficients of the Newton interpolating polynomial $p(x)$.

Adding new data (x_{n+1}, f_{n+1}) means adding more row at the bottom of the table. As each divided difference is calculated in 3 flops, this can be done with $\mathcal{O}(n)$ additional operations.

Divided differences table

Example: The divided difference table for the data points (0, 3), (1, 4), (2, 7) and (4, 19) is

x	f				
0	3				
1	4	$\frac{4-3}{1-0} = 1$			
2	7	$\frac{7-4}{2-1} = 3$	$\frac{3-1}{2-0} = 1$		
4	19	$\frac{19-7}{4-2} = 6$	$\frac{6-3}{4-1} = 1$	$\frac{1-1}{4-0} = 0$	

Divided differences table

Example: The divided difference table for the data points (0, 3), (1, 4), (2, 7) and (4, 19) is

x	f				
0	3				
1	4	$\frac{4-3}{1-0} = 1$			
2	7	$\frac{7-4}{2-1} = 3$	$\frac{3-1}{2-0} = 1$		
4	19	$\frac{19-7}{4-2} = 6$	$\frac{6-3}{4-1} = 1$	$\frac{1-1}{4-0} = 0$	

The Newton interpolating polynomial is given by

$$p(x) = 3 + 1 \cdot (x-0) + 1 \cdot (x-0)(x-1) + 0 \cdot (x-0)(x-1)(x-2) = 3 + x^2.$$

Divided differences table

If the point (5, 22) is added to the data, then the updated table is:

x	f				
0	3				
1	4	$\frac{4-3}{1-0} = 1$			
2	7	$\frac{7-4}{2-1} = 3$	$\frac{3-1}{2-0} = 1$		
4	19	$\frac{19-7}{4-2} = 6$	$\frac{6-3}{4-1} = 1$	$\frac{1-1}{4-0} = 0$	
5	22	$\frac{22-19}{5-4} = 3$	$\frac{3-6}{5-2} = -1$	$\frac{-1-1}{5-1} = -\frac{1}{2}$	$\frac{-\frac{1}{2}-0}{5-0} = -\frac{1}{10}$

The Newton interpolating polynomial is given by

$$q(x) = p(x) - \frac{1}{10}(x-0)(x-1)(x-2)(x-4) = x^4 - 7x^3 + 15x^2 - 8x + 3.$$

Newton polynomial via divided differences

Theorem: Let $p(x) = a_0N_0(x) + \cdots + a_nN_n(x)$ be such that $p(x_j) = f_j$ for $j = 0 : n$. Then

$$a_j = f[x_0, x_1, \dots, x_j] \text{ for } j = 0 : n.$$

Proof: The result is true for $n = 0$. Assume that the result is true for Newton interpolating polynomials of degree $\leq n - 1$.

Newton polynomial via divided differences

Theorem: Let $p(x) = a_0N_0(x) + \cdots + a_nN_n(x)$ be such that $p(x_j) = f_j$ for $j = 0 : n$. Then

$$a_j = f[x_0, x_1, \dots, x_j] \text{ for } j = 0 : n.$$

Proof: The result is true for $n = 0$. Assume that the result is true for Newton interpolating polynomials of degree $\leq n - 1$.

Let $q(x) = \sum_{j=0}^{n-1} b_j N_j(x)$ be the interpolating polynomial for the data $(x_1, f_1), \dots, (x_n, f_n)$ and $s(x) = \sum_{j=0}^{n-1} c_j N_j(x)$ be the interpolating polynomial for the data $(x_0, f_0), \dots, (x_{n-1}, f_{n-1})$.

Newton polynomial via divided differences

Theorem: Let $p(x) = a_0N_0(x) + \cdots + a_nN_n(x)$ be such that $p(x_j) = f_j$ for $j = 0 : n$. Then

$$a_j = f[x_0, x_1, \dots, x_j] \text{ for } j = 0 : n.$$

Proof: The result is true for $n = 0$. Assume that the result is true for Newton interpolating polynomials of degree $\leq n - 1$.

Let $q(x) = \sum_{j=0}^{n-1} b_j N_j(x)$ be the interpolating polynomial for the data $(x_1, f_1), \dots, (x_n, f_n)$ and $s(x) = \sum_{j=0}^{n-1} c_j N_j(x)$ be the interpolating polynomial for the data $(x_0, f_0), \dots, (x_{n-1}, f_{n-1})$.

By induction hypothesis $b_{n-1} = f[x_1, \dots, x_n]$ and $c_{n-1} = f[x_0, \dots, x_{n-1}]$.

Note that $r(x) := q(x) + \frac{x-x_n}{x_n-x_0}(q(x) - s(x))$ is the interpolating polynomial for the data $(x_0, f_0), \dots, (x_n, f_n)$. (Check)

Newton polynomial via divided differences

Theorem: Let $p(x) = a_0N_0(x) + \cdots + a_nN_n(x)$ be such that $p(x_j) = f_j$ for $j = 0 : n$. Then

$$a_j = f[x_0, x_1, \dots, x_j] \text{ for } j = 0 : n.$$

Proof: The result is true for $n = 0$. Assume that the result is true for Newton interpolating polynomials of degree $\leq n - 1$.

Let $q(x) = \sum_{j=0}^{n-1} b_j N_j(x)$ be the interpolating polynomial for the data $(x_1, f_1), \dots, (x_n, f_n)$ and $s(x) = \sum_{j=0}^{n-1} c_j N_j(x)$ be the interpolating polynomial for the data $(x_0, f_0), \dots, (x_{n-1}, f_{n-1})$.

By induction hypothesis $b_{n-1} = f[x_1, \dots, x_n]$ and $c_{n-1} = f[x_0, \dots, x_{n-1}]$.

Note that $r(x) := q(x) + \frac{x-x_n}{x_n-x_0}(q(x) - s(x))$ is the interpolating polynomial for the data $(x_0, f_0), \dots, (x_n, f_n)$. (Check)

By uniqueness, $r(x) = p(x)$. Equating the coefficients of x^n , we have

$$a_n = \frac{f[x_1, x_2, \dots, x_n] - f[x_0, x_1, \dots, x_{n-1}]}{x_n - x_0} = f[x_0, x_1, \dots, x_n]. \blacksquare$$

Summary

For the data $(x_0, f_0), \dots, (x_n, f_n)$, there is a unique $p(x) \in \mathcal{P}_n$ given by

- Vandermonde interpolating polynomial: $p(x) = \sum_{j=0}^n a_j x^j$.
- Lagrange interpolating polynomial: $p(x) = \sum_{j=0}^n \ell_j(x) f_j$.
- Barycentric Lagrange: $p(x) = \frac{\sum_{j=0}^n \frac{w_j f_j}{x - x_j}}{\sum_{j=0}^n \frac{w_j}{x - x_j}}$.
- Newton interpolating polynomial:

$$p(x) = \sum_{j=0}^n f[x_0, \dots, x_j] (x - x_0) \cdots (x - x_{j-1}).$$

Summary

For the data $(x_0, f_0), \dots, (x_n, f_n)$, there is a unique $p(x) \in \mathcal{P}_n$ given by

- **Vandermode interpolating polynomial:** $p(x) = \sum_{j=0}^n a_j x^j$.
- **Lagrange interpolating polynomial:** $p(x) = \sum_{j=0}^n \ell_j(x) f_j$.
- **Barycentric Lagrange:** $p(x) = \frac{\sum_{j=0}^n \frac{w_j f_j}{x - x_j}}{\sum_{j=0}^n \frac{w_j}{x - x_j}}$.
- **Newton interpolating polynomial:**

$$p(x) = \sum_{j=0}^n f[x_0, \dots, x_j] (x - x_0) \cdots (x - x_{j-1}).$$

Example: For the data set $(-2, -27), (0, -1), (1, 0)$, we have the interpolating polynomials in various forms:

Vandermode: $p(x) = -1 + 5x - 4x^2$.

Lagrange: $p(x) = -\frac{9}{2}x(x-1) + \frac{1}{2}(x+2)(x-1)$.

Newton: $p(x) = -27 + 13(x+2) - 4(x+2)x$
